VCVio/OracleComp/SimSemantics/QueryTracking/CountingOracle.lean
@@ -11,39 +11,60 @@ import VCVio.OracleComp.SimSemantics.Simulate
 This file defines a simulation oracle `countingOracle` for counting the number of queries made
 while running the computation. The count is represented by a function from oracle indices to
 counts, allowing each oracle to be tracked individually.
+
+Tracking individually is not necessary, but gives tighter security bounds in some cases.
+It also allows for generating things like seed values for a computation more tightly.
 -/
-
-open OracleComp
-
--- namespace OracleSpec
-
--- @[inline, reducible]
--- def QueryCount (spec : OracleSpec) : Type := spec.ι → ℕ
-
--- variable {spec : OracleSpec}
-
--- def QueryCount.increment (qc : spec.QueryCount) (i : spec.ι) (n : ℕ) : spec.QueryCount :=
---   Function.update qc i (qc i + n)
-
--- def QueryCount.decrement (qc : spec.QueryCount) (i : spec.ι) (n : ℕ) : spec.QueryCount :=
---   Function.update qc i (qc i - n)
-
--- instance : Zero (QueryCount spec) := ⟨λ _ ↦ 0⟩
-
--- end OracleSpec
 
 open OracleComp OracleSpec Function
 
-def countingOracle {ι : Type} [DecidableEq ι]
-    {spec : OracleSpec ι} : spec →[ι → ℕ]ₛₒ spec :=
+/-- Oracle for counting the number of queries made by a computation. The count is stored as a
+function from oracle indices to counts, to give finer grained information about the count. -/
+def countingOracle {ι : Type} [DecidableEq ι] {spec : OracleSpec ι} :
+    spec →[ι → ℕ]ₛₒ spec :=
   λ i t qc ↦ (·, update qc i (qc i + 1)) <$> query i t
 
 namespace countingOracle
 
-variable {ι : Type} [DecidableEq ι] {spec : OracleSpec ι}
+variable {ι : Type} [DecidableEq ι] {spec : OracleSpec ι} {α β γ : Type}
 
 @[simp]
 lemma apply_eq (i : ι) (t : spec.domain i) :
     countingOracle i t = λ qc ↦ (·, update qc i (qc i + 1)) <$> query i t := rfl
+
+/-- We can always reduce the initial state of simulation with a counting oracle to start with a
+count of zero, and add the initial count back on at the end. -/
+lemma support_simulate (oa : OracleComp spec α) (qc : ι → ℕ) :
+    (simulate countingOracle qc oa).support =
+      Prod.map id (qc + ·) '' (simulate countingOracle 0 oa).support := by
+  revert qc
+  induction oa using OracleComp.inductionOn with
+  | h_pure a => simp
+  | h_queryBind i t oa hoa =>
+      refine λ qc ↦ ?_
+      simp only [simulate_bind, simulate_query, apply_eq, support_bind, support_map, support_query,
+        Set.image_univ, Set.mem_range, Set.iUnion_exists, Set.iUnion_iUnion_eq', Prod.map_apply,
+        id_eq, Pi.zero_apply, zero_add, Set.image_iUnion]
+      refine Set.iUnion_congr (λ u ↦ ?_)
+      simp only [hoa u (update qc i (qc i + 1)), hoa u (update 0 i 1),
+        ← Set.image_comp, Function.comp, Prod.map_apply, id_eq, ← add_assoc]
+      refine Set.image_congr' (λ z ↦ Prod.eq_iff_fst_eq_snd_eq.2 ⟨rfl, funext (λ j ↦ ?_)⟩)
+      by_cases hij : j = i <;> simp [hij, add_assoc]
+
+/-- Reduce membership in the support of simulation with counting to membership in simulation
+starting with the count at `0`.
+TODO: lemmas like this suggest maybe support shouldn't auto reduce on the computation type? -/
+lemma mem_support_simulate_iff_exists (oa : OracleComp spec α) (qc : ι → ℕ) (z : α × (ι → ℕ)) :
+    z ∈ (simulate countingOracle qc oa).support ↔
+      ∃ qc', (z.1, qc') ∈ (simulate countingOracle 0 oa).support ∧ qc + qc' = z.2 := by
+  rw [support_simulate]
+  simp only [Prod.map_apply, id_eq, Set.mem_image, Prod.eq_iff_fst_eq_snd_eq, Prod.exists]
+  refine ⟨λ h ↦ let ⟨x, qc', h, hx, hqc'⟩ := h; ⟨qc', hx ▸ ⟨h, hqc'⟩⟩,
+    λ h ↦ let ⟨qc', h, hqc'⟩ := h; ⟨z.1, qc', h, rfl, hqc'⟩⟩
+
+lemma le_of_mem_support_simulate (oa : OracleComp spec α) (qc : ι → ℕ) (z : α × (ι → ℕ))
+    (h : z ∈ (simulate countingOracle qc oa).support) : qc ≤ z.2 := by
+  rw [mem_support_simulate_iff_exists] at h
+  exact let ⟨qc', _, h⟩ := h; h ▸ le_self_add
 
 end countingOracle
