VCVio/OracleComp/SimSemantics/QueryTracking/LoggingOracle.lean
@@ -10,28 +10,35 @@ import VCVio.OracleComp.SimSemantics.Simulate
 
 -/
 
+variable {ι : Type} [DecidableEq ι] {spec : OracleSpec ι} {α β : Type}
+
 namespace OracleSpec
 
 /-- Log of oracle queries represented by lists of input output pairs,
 parameterized by the set of oracles available. -/
-def QueryLog {ι : Type} (spec : OracleSpec ι) : Type :=
+def QueryLog (spec : OracleSpec ι) : Type :=
   (i : ι) → List (spec.domain i × spec.range i)
 
-variable {ι : Type}
+namespace QueryLog
+
+section logQuery
 
 /-- Update a query log by adding a new element to the appropriate list.
 Note that this requires decidable equality on the indexing set. -/
-def QueryLog.logQuery [DecidableEq ι] {spec : OracleSpec ι} (log : QueryLog spec) {i : ι}
+def logQuery  (log : QueryLog spec) {i : ι}
     (t : spec.domain i) (u : spec.range i) : QueryLog spec :=
   Function.update log i ((t, u) :: log i)
 
+end logQuery
+
 /-- Check if an element was ever queried in a log of queries.
 Relies on decidable equality of the domain types of oracles. -/
-def QueryLog.wasQueried {spec : OracleSpec ι} (log : QueryLog spec)
-    (i : ι) (t : spec.domain i) : Bool :=
+def wasQueried (log : QueryLog spec) (i : ι) (t : spec.domain i) : Bool :=
   match (log i).find? (λ (t', _) ↦ t = t') with
   | Option.some _ => true
   | Option.none => false
+
+end QueryLog
 
 end OracleSpec
 
@@ -40,6 +47,14 @@ open OracleComp OracleSpec
 /-- Simulation oracle for tracking the quries in a `QueryLog`, without modifying the actual
 behavior of the oracle. Requires decidable equality of the indexing set to determine
 which list to update when queries come in. -/
-def loggingOracle {ι : Type} [DecidableEq ι] {spec : OracleSpec ι} :
-    spec →[QueryLog spec]ₛₒ spec :=
+def loggingOracle : spec →[QueryLog spec]ₛₒ spec :=
   λ i t log ↦ do let u ← query i t; return (u, log.logQuery t u)
+
+namespace loggingOracle
+
+@[simp]
+lemma apply_eq (i : ι) (t : spec.domain i) (log : QueryLog spec) :
+    loggingOracle i t log = do let u ← query i t; return (u, log.logQuery t u) := rfl
+
+
+end loggingOracle
