VCVio/OracleComp/SimSemantics/QueryTracking/RandOracle.lean
@@ -1,0 +1,54 @@
+/-
+Copyright (c) 2024 Devon Tuma. All rights reserved.
+Released under Apache 2.0 license as described in the file LICENSE.
+Authors: Devon Tuma
+-/
+import VCVio.OracleComp.SimSemantics.QueryTracking.CachingOracle
+
+/-!
+# Random Oracles
+
+This file defines a simulation oracle `randOracle` that uniformly responds to fresh queries,
+but caches previous queries for future calls.
+
+Implemented as a composition of caching and uniform oracles,
+with the state of the uniform oracle masked away.
+-/
+
+open OracleSpec OracleComp
+
+variable {ι : Type} [DecidableEq ι] {spec : OracleSpec ι} [∀ i, SelectableType (spec.range i)]
+  {α β γ : Type}
+
+/-- Random oracles as a composition of a uniform oracle with a caching oracle. -/
+def randOracle {ι : Type} [DecidableEq ι] {spec : OracleSpec ι}
+    [∀ i, SelectableType (spec.range i)] : spec →[QueryCache spec]ₛₒ unifSpec :=
+  (unifOracle ∘ₛₒ cachingOracle).maskState (Equiv.prodPUnit (QueryCache spec))
+
+namespace randOracle
+
+/-- Executing a random oracle is the same as lookuping up the value and choosing a uniformly
+random new value if it doesn't already exist. -/
+@[simp]
+lemma apply_eq (i : ι) (t : spec.domain i) (cache : QueryCache spec) :
+    randOracle i t cache = cache.lookup_or_else i t ($ᵗ spec.range i) := by
+  simp only [randOracle, SimOracle.maskState_apply, Equiv.prodPUnit_symm_apply,
+    SimOracle.compose_apply, cachingOracle.apply_eq, QueryCache.lookup_or_else, Functor.map_map,
+    Function.comp, Prod.map_apply, id_eq, Equiv.prodPUnit_apply, Prod.mk.eta]
+  cases cache i t
+  · simp [map_eq_bind_pure_comp]
+  · simp
+
+/-- Simulation with a random oracle looks like choosing a random function and answering queries
+with that. TODO: there's some tricky things in the induction step here. -/
+lemma evalDist_simulate'_eq_uniformSelect_fun_bind
+    [Inhabited γ] [Fintype γ] [Fintype β] [DecidableEq β]
+    [DecidableEq γ] [SelectableType γ]
+    [SelectableType (β → γ)]
+    (oa : OracleComp (β →ₒ γ) α) :
+    [simulate' randOracle ∅ oa] = [do
+      let f ←$ᵗ (β → γ)
+      simulate' (λ () t () ↦ return (f t, ())) () oa] := by
+  sorry
+
+end randOracle
